TODO.v
@@ -1,0 +1,83 @@
+From Coq Require Import Arith.Arith.
+From Coq Require Import Lists.List.
+From Coq Require Import Lia.
+
+From Elo Require Import Map.
+From Elo Require Import Properties.
+From Elo Require Import Lemmas.
+From Elo Require Import Preservation.
+From Elo Require Import PtrTyp.
+From Elo Require Import Soundness.
+From Elo Require Import Multistep.
+
+Inductive has_address (ad : addr) : tm  -> Prop :=
+  | ha_ref : forall T,
+    has_address ad <{&ad :: T}>
+
+  | ha_new : forall T t,
+    has_address ad t ->
+    has_address ad <{new T t}>
+
+  | ha_load : forall t,
+    has_address ad t ->
+    has_address ad <{*t}>
+
+  | ha_asg1 : forall t1 t2,
+    has_address ad t1 ->
+    has_address ad <{t1 = t2}>
+
+  | ha_asg2 : forall t1 t2,
+    has_address ad t2 ->
+    has_address ad <{t1 = t2}>
+
+  | ha_fun : forall x T t,
+    has_address ad t ->
+    has_address ad <{fn x T t}>
+
+  | ha_call1 : forall t1 t2,
+    has_address ad t1 ->
+    has_address ad <{call t1 t2}>
+
+  | ha_call2 : forall t1 t2,
+    has_address ad t2 ->
+    has_address ad <{call t1 t2}>
+
+  | ha_seq1 : forall t1 t2,
+    has_address ad t1 ->
+    has_address ad <{t1; t2}>
+
+  | ha_seq2 : forall t1 t2,
+    has_address ad t2 ->
+    has_address ad <{t1; t2}>
+  .
+
+Lemma ha_dec : forall ad t,
+  Decidable.decidable (has_address ad t).
+Proof.
+  unfold Decidable.decidable. intros. induction t;
+  try solve
+    [ right; intros F; inv F
+    | try (destruct IHt || destruct IHt1, IHt2) ; solve
+        [ left; eauto using has_address
+        | right; intros F; inv F; contradiction
+        ]
+    ].
+  destruct (nat_eq_dec ad n); subst; eauto using has_address.
+  right. intros F. inv F. contradiction.
+Qed.
+
+Lemma ha_then_acc : forall ad m t,
+  has_address ad t -> access ad m t.
+Proof.
+  intros * Hha. induction Hha; eauto using access.
+Qed.
+
+Lemma acc'_dec : forall ad m t,
+  Decidable.decidable (access ad m t).
+Proof.
+  unfold Decidable.decidable. intros.
+  assert (Decidable.decidable (has_address ad t)) as [? | ?]
+    by eauto using ha_dec;
+  eauto using ha_then_acc.
+  (* has_address ad' t /\ access ad m m[ad'] *)
+Abort.
